## Билет 27

### Формула обращения Мёбиуса. Аддитивный вариант

#### Теорема 20

Пусть $f, g : \mathbb{N} \to \mathbb{R}$, причем $\displaystyle f(m) = \sum_{d \mid m} g(d)$. Тогда $\displaystyle g(m)= \sum_{n|m}\mu(\frac{m}{n})f(n)$

**Доказательство.**

$$
\sum_{n \mid m} \mu\left(\frac{m}{n}\right) f(n) = \sum_{n \mid m} \mu\left(\frac{m}{n}\right) \times \sum_{d \mid n} g(d) = \sum_{d \mid m} \left( (g(d) \times \sum_{d \mid n \mid m} \mu\left(\frac{m}{n}\right)\right)
$$

по [Лемме 8](#Лемма-8).

$$
\sum_{d \mid n \mid m} \mu\left(\frac{m}{n}\right) = 
\begin{cases} 
1, & \text{если } m = d, \\
0, & \text{если } m > d.
\end{cases}
$$

Таким образом,

$$
\sum_{n \mid m} \mu\left(\frac{m}{n}\right) f(n) = g(m).
$$
