## Билет 29

### Формула обращения Мёбиуса. Мультипликативный вариант

#### Теорема 22

Пусть $K$ — поле, $f, g : \mathbb{N} \to K \setminus \{0\}$, причем $\displaystyle f(m) = \prod_{n \mid m} g(d)$. Тогда $\displaystyle g(m) = \prod_{n \mid m} f(n)^{\mu\left(\frac{m}{n}\right)}$.

#### Доказательство

$$
\prod_{n \mid m} f(n)^{ \mu\left(\frac{m}{n}\right)} = \prod_{n \mid m} \left( \prod_{d \mid n} g(d) \right)^{\mu\left(\frac{m}{n}\right)} =
$$

$$
= \prod_{d \mid m} g(d)^{ \displaystyle \sum_{d \mid n \mid m} \mu\left(\frac{m}{n}\right)}
$$

$$
= g(m)
$$

по [Лемме 8](#Лемма-8).
